{-# OPTIONS --rewriting #-}

open import Agda.Builtin.Nat
open import Agda.Builtin.Equality
open import Agda.Builtin.Equality.Rewrite

variable
    m n : Nat

cong : ∀ { a b} { A : Set a }  { B : Set b }
       (f : A → B ) {m  n}  → m ≡ n → f m ≡ f n
cong f refl = refl

+zero : m + zero ≡ m
+zero {m = zero}  = refl
+zero {m = suc m} = cong suc +zero

+suc : m + (suc n) ≡ suc (m + n)
+suc {m = zero}  = refl
+suc {m = suc m} = cong suc +suc

{-# REWRITE +zero +suc #-}

test : ( m + m + 1 + n + 1 ≡ 2 + (n + m) + m )
test = refl
